LeanC/Arrays.lean
@@ -1,0 +1,66 @@
+import LeanC.Types
+/-!
+# Array Types for lean_c
+
+This module defines core RAM related types:
+
+CMemoryBlock -- represents pointer to void, but with associated
+allocated size to guarantee within bounds operations.
+
+CArray -- MemoryBlock with Associated Type
+
+CSlice -- a subarray (Rust inspired name)
+
+In general we need a proof system that the block of memory is allocated.
+The guarantee can be obtained by generating allocation call as a result of the
+construction operator, but we need to take into account that allocation can fail.
+Conceptually, both branches -- successive allocation and failed allocation should be
+processed.
+
+we can have either smart or private constructors.
+-/
+
+namespace LeanC
+universe u
+
+/-- For fixed size memory blocks we know the allocated size
+so we can supply it with the parameter
+-/
+inductive CFixedSizeMemoryBlock (n:Nat) where
+| mk
+
+/-- For dynamically allocated memory block we need a variable that will store
+the allocated size, so we need a reference to the variable.
+Roughly speaking this only possible after we define Variables, and references to variables.
+-/
+inductive CDynamicMemoryBlock where
+| mk
+
+
+/-- CMemoryBlock represents allocated memory block
+It is technically equivalent to (void *) type with allocated size information.
+It represents succesifully allocated block of RAM
+Technically Mempory block can be an argument of f(void *)
+
+There are 2 way to allocate memory:
+- we can have a fixed size allocation known at compile time
+- dynamic allocations, we need a variable storing actual value
+-/
+inductive CMemoryBlock (α:Type u) where
+| mk
+
+/-- CArray_t represents a C array type.
+
+CArray has element type and size. It is usually stack allocated, when declared.
+However we can define a pointer to an array type as well. This can be in heap, but we indicate that
+each array has fixed size.
+-/
+inductive CArray_t (α : Type u) [IsCType α] where
+  | mk : Nat → CArray_t α
+instance (α : Type u) [IsCType α] : IsCType (CArray_t α) where
+  isCType := True
+instance (α : Type u) [IsCType α] : IsCFuncArgType (CArray_t α) where
+  isCFuncArgType := True
+
+
+end LeanC
